Added 'parent' pointer to nodes

BST.dfy
@@ -4,35 +4,41 @@
 // JAVA REFERENCE: https://github.com/dtfiedler/java-binary-tree/blob/master/src/BinaryTree.java
 
 /*
-    [Lucas]:
-
-    TODO: DOUBLE CHECK LUCAS' IMPLEMENTATIONS FOR INSERT AND FIND, ENSURE VALIDITY HOLDS
+    TODO: DOUBLE CHECK IMPLEMENTATION & VERIFICATION FOR INSERT 
+    TODO: IMPLEMENT & VERIFY FIND FUNCTIONS
     TODO: IMPLEMENT & VERIFY DELETE FUNCTION
     TODO: IMPLEMENT & VERIFY TREE TRAVERSALS
+
+    Something that could maybe help with the above tasks is to also create a function that traverses the tree and outputs the values, in sorted order, in an array.
+    This could make it easier to verify
 */
 
-datatype Tree = Null | Node(left: Tree, value: int, right: Tree)
+datatype Tree = Null | Node(left: Tree, value: int, right: Tree, parent: Tree)
 
 class BST{
     var root: Tree
 
-    constructor(r: Tree) 
-        ensures isBST(r) ==> isBST(root)
+    constructor(r: Tree)
+        ensures isBST(root)
     {
-        root := r;
+       root := r;
+       new; 
+       if (!isBST(r)) {
+        root := Null; // Constructs valid tree, on the condition that paramter r is also valid
+       }
     }
 
     // Used as helper in isBST
     function max_value_in_tree(t: Tree): int
         requires t != Null
+        
     {
         match t
-            case Node(_, v, r_child) => 
+            case Node(_, v, r_child, _) => 
                 if r_child == Null then
                     v
                 else 
                     max_value_in_tree(r_child)
-                
     }
 
 
@@ -41,7 +47,7 @@ class BST{
         requires t != Null
     {
         match t
-            case Node(l_child, v, _) => 
+            case Node(l_child, v, _, _) => 
                 if l_child == Null then
                     v
                 else 
@@ -49,12 +55,11 @@ class BST{
                 
     }
 
-    // [Lucas]: Fixed the inverted condition and renamed for clarity.
     predicate in_BST(t: Tree, search_val: int)
     {
         match t
             case Null => false
-            case Node(l, node_val, r) =>
+            case Node(l, node_val, r, _) =>
                 if node_val == search_val then
                     true
                 else if search_val < node_val then
@@ -63,14 +68,14 @@ class BST{
                     in_BST(r, search_val)
     }
 
-    // [Lucas]: Fixed to verify fully. Strengthened ensures to iff, removed unreachable Null case, removed assumes, renamed for clarity.
+    // Returns true iff 't' contains search_val
     method value_in_tree(t: Tree, search_val: int) returns (ret: bool)
         requires t != Null
         ensures ret ==> in_BST(t, search_val) // ENSURE THAT THE VALUE IS IN THE TREE IFF THE PREDICATE HOLDS
         decreases t
     {
         match t
-            case Node(l_child, node_val, r_child) => 
+            case Node(l_child, node_val, r_child, _) => 
                 if (node_val == search_val) {
                     ret := true;
                 } else if (search_val < node_val) { // LESS THAN CASE
@@ -88,41 +93,70 @@ class BST{
                 }
     }
 
-    function isBST(t: Tree): bool
+    // True iff all values in t are < bound
+    predicate all_less_than(t: Tree, bound: int)
+    {
+      match t
+      case Null => true
+      case Node(l, v, r, _) =>
+        v < bound && all_less_than(l, bound) && all_less_than(r, bound)
+    }
+
+    // True iff all values in t are > bound
+    predicate all_greater_than(t: Tree, bound: int)
+    {
+      match t
+      case Null => true
+      case Node(l, v, r, _) =>
+        v > bound && all_greater_than(l, bound) && all_greater_than(r, bound)
+    }
+
+    // TODO: ENSURE THAT THESE CONDITIONS ACTUALLY DO ENFORCE THE ORDERING PROPERTY (because I'm actually not even sure if it does)
+    predicate isBST(t: Tree)
     {
         match t
             case Null => true
-            case Node(l_child,_,r_child) => 
-               isBST(l_child) && isBST(r_child) && (l_child != Null ==> max_value_in_tree(l_child) < t.value) && (r_child != Null ==> min_value_in_tree(r_child) > t.value)
+            case Node(l_child,v,r_child, _) => 
+                isBST(l_child) 
+                && isBST(r_child) 
+                // && (l_child != Null ==> max_value_in_tree(l_child) <= t.value) 
+                // && (r_child != Null ==> min_value_in_tree(r_child) >= t.value)
+                && if (t.parent != Null) then (t == t.parent.left ==> t.value < t.parent.value) && (t == t.parent.right ==> t.value > t.parent.value) else true
+                && (l_child != Null ==> all_less_than(l_child, v))
+                && (r_child != Null ==> all_greater_than(r_child, v))
     }
 
-    // [Lucas]:
     // Appends a new value, v, as a descendent of current_node
     // TODO : ENSURE PROPER ORDERING AS POST CONDITION
     // TODO : ADD ANY OTHER APPROPRIATE VERIFICATION CONDITIONS 
     method add_recursive(current_node: Tree, v: int) returns (ret: Tree)
         requires isBST(current_node)
         ensures isBST(ret)
+        ensures in_BST(ret, v)
     {
-        if (current_node == Null) {
-            ret := Node(Null, v, Null);
-        } else {
-            if (v < current_node.value) { // Insert as left child
-                ret := add_recursive(current_node.left, v);
+        match current_node
+        case Node(curr_l, curr_v, curr_r, _) =>
+            if (v < curr_v) { // Insert as left child
+                var tmp := add_recursive(current_node.left, v);
+                ret := Node(tmp, curr_v, curr_r, current_node);
             }
-            else { // Insert as right child
-                ret := add_recursive(current_node.right, v);
+            else if (v > curr_v) { // Insert as right child
+                var tmp := add_recursive(current_node.right, v);
+                ret := Node(curr_l, curr_v, tmp, current_node);
+            } else {
+                ret := current_node;
             }
-        }
+        case Null =>
+            ret := Node(Null, v, Null, current_node);
     }
 
-    // [Lucas]:
     // So far, we just assume that we have a valid structure, and then that insertion doesn't break our structure
     // TODO: FIND A WAY TO VERIFY THAT, FROM THE VERY BEGINNING, THE BST PROPERTIES HOLD
     method insert(v: int)
+        modifies this
         requires isBST(this.root)
         ensures isBST(this.root)
-        modifies this
+
     {
         this.root := add_recursive(this.root, v);
     }
